heap_lang/tactics.v
@@ -183,10 +183,20 @@ Definition atomic (e : expr) :=
   | App (Rec _ _ (Lit _)) (Lit _) => true
   | _ => false
   end.
-Lemma atomic_correct e : atomic e → heap_lang.atomic (to_expr e).
+Lemma atomic_correct e : atomic e → ectx_language.atomic (to_expr e).
 Proof.
-  destruct e; simpl; repeat (case_match; try done);
-    naive_solver eauto using to_val_is_Some.
+  intros He. split.
+  - intros σ e' σ' ef.
+    destruct e; simpl; try done; repeat (case_match; try done);
+    inversion 1; rewrite ?to_of_val; eauto. subst.
+    unfold subst'; repeat (case_match || contradiction || simplify_eq/=); eauto.
+  - intros K e' Hfill Hnotval. destruct K as [|Ki K]; [done|exfalso].
+    apply (fill_not_val K), eq_None_not_Some in Hnotval. apply Hnotval. simpl.
+    revert He. destruct e; simpl; try done; repeat (case_match; try done);
+    rewrite ?bool_decide_spec;
+    destruct Ki; inversion Hfill; subst; clear Hfill;
+    try naive_solver eauto using to_val_is_Some.
+    move=> _ /=; destruct decide as [|Nclosed]; [by eauto | by destruct Nclosed].
 Qed.
 End W.
 
@@ -214,16 +224,15 @@ Ltac solve_to_val :=
 
 Ltac solve_atomic :=
   try match goal with
-  | |- context E [language.atomic ?e] =>
-     let X := context E [atomic e] in change X
+  | |- language.atomic ?e => apply ectx_language_atomic
   end;
   match goal with
-  | |- atomic ?e =>
+  | |- ectx_language.atomic ?e =>
      let e' := W.of_expr e in change (atomic (W.to_expr e'));
      apply W.atomic_correct; vm_compute; exact I
   end.
-Hint Extern 0 (atomic _) => solve_atomic : fsaV.
 Hint Extern 0 (language.atomic _) => solve_atomic : fsaV.
+Hint Extern 0 (ectx_language.atomic _) => solve_atomic : fsaV.
 
 (** Substitution *)
 Ltac simpl_subst :=
